fairness/heap_lang/model_logic.v
@@ -4,6 +4,8 @@ From iris.base_logic Require Export gen_heap.
 From trillium.fairness.heap_lang Require Import tactics notation sswp_logic.
 From trillium.fairness Require Import fairness resources fuel model_plug lm_fair.
 From trillium.fairness.lm_rules Require Import model_step resources_updates fuel_step.
+From iris.proofmode Require Import coq_tactics reduction spec_patterns.
+From iris.proofmode Require Export tactics.
 
 
 Section LMLocalRules.
@@ -20,13 +22,15 @@ Section LMLocalRules.
   Let msi: fmstate LF -> iProp Σ := model_state_interp (LM := iLM).
 
   Context {lifted_roles: fmstate LF -> gset (fmrole LF)}.
-  Hypothesis (IMPL_LIFT: forall (δ δ': fmstate LF),
-                 dom (ls_tmap δ') = dom (ls_tmap δ) ->
-                 live_roles _ δ' ⊆ live_roles _ δ ->
-                 lifted_roles δ' ⊆ lifted_roles δ).
-  Hypothesis (TRANS_NO_ENAB: forall δ g δ',
-                 locale_trans δ g δ' (LM := iLM) ->
-                 live_roles LF δ' ⊆ live_roles LF δ). 
+  Hypothesis (IMPL_LIFT: forall (δ1 δ2: fmstate LF) g R2,
+                 (* dom (ls_tmap δ') = dom (ls_tmap δ) -> *)
+                 (* live_roles _ δ' ⊆ live_roles _ δ -> *)
+                 locale_trans δ1 g δ2 (LM := iLM) ->
+                 ls_tmap δ2 = <[g:=R2]> (ls_tmap δ1) ->
+                 lifted_roles δ2 ⊆ lifted_roles δ1).
+  (* Hypothesis (TRANS_NO_ENAB: forall δ g δ', *)
+  (*                locale_trans δ g δ' (LM := iLM) -> *)
+  (*                live_roles LF δ' ⊆ live_roles LF δ).  *)
   
   Let lm_local_rule := local_rule (msi := msi) (lifted_roles := lifted_roles). 
   
@@ -55,11 +59,9 @@ Section LMLocalRules.
     iPureIntro.
     assert (fmtrans LF δ (Some ζ) δ2) as STEP'. 
     { simpl. eexists. split; [apply STEP| ]. done. }
-    split; [done| ].    
-    apply IMPL_LIFT.
-    - rewrite TM. rewrite dom_insert_L. 
-      apply locale_trans_dom in STEP'. clear -STEP'. set_solver.
-    - eapply TRANS_NO_ENAB. apply STEP'.
+    split; [done| ].
+    eapply IMPL_LIFT; eauto.
+    apply STEP'. 
   Qed.
 
   Lemma fuel_keep_step_local_rule fs ζ:
@@ -79,9 +81,11 @@ Section LMLocalRules.
     assert (fmtrans LF δ (Some ζ) δ2) as STEP'. 
     { simpl. eexists. split; [apply STEP| ]. done. }
     split; [done| ].
-    apply IMPL_LIFT.
-    - by rewrite TM.
-    - eapply TRANS_NO_ENAB. apply STEP'.
+    pose proof STEP' as [foo bar]%locale_trans_dom%elem_of_dom. 
+    eapply IMPL_LIFT; eauto.
+    { apply STEP'. }
+    rewrite TM. symmetry.
+    by apply insert_id.
   Qed.
 
   Lemma fuel_drop_step_local_rule rem s fs ζ:
@@ -105,13 +109,13 @@ Section LMLocalRules.
     assert (fmtrans LF δ (Some ζ) δ2) as STEP'. 
     { simpl. eexists. split; [apply STEP| ]. done. }
     split; [done| ].
-    apply IMPL_LIFT.
-    - rewrite TM. rewrite dom_insert_L. 
-      apply locale_trans_dom in STEP'. clear -STEP'. set_solver.
-    - eapply TRANS_NO_ENAB. apply STEP'.
+    eapply IMPL_LIFT; eauto.
+    apply STEP'. 
   Qed. 
 
 End LMLocalRules.  
+
+
 
 
 Section ModelLogic.
@@ -164,7 +168,46 @@ Section ModelLogic.
     iApply wp_value. iFrame.
   Qed.
 
+Section Tactics.
+
+    (* From trillium.program_logic Require Import ectxi_language.  *)
+
+
+
+  Lemma tac_cwp_bind
+    (* K Δ s E Φ e f : *)
+    (* f = (λ e, fill K e) → (* as an eta expanded hypothesis so that we can `simpl` it *) *)
+    (* envs_entails Δ (WP e @ s; E {{ v, WP f (Val v) @ s; E {{ Φ }} }})%I → *)
+    (* envs_entails Δ (WP fill K e @ s; E {{ Φ }}). *)
+K Δ (e: expr heap_lang) (Φ: val heap_lang -> iProp Σ) (s: stuckness) (ε__wp ε__lift: coPset) (τ: locale heap_lang) (ρ: fmrole M) f:
+    f = (λ e, fill K e) ->
+      envs_entails Δ (CWP e (fun v => CWP (f (Val v)) Φ s ε__wp ε__lift τ ρ) s ε__wp ε__lift τ ρ) ->
+      envs_entails Δ (CWP (fill K e) Φ s ε__wp ε__lift τ ρ). 
+  Proof. rewrite envs_entails_unseal=> -> ->. by apply: cwp_bind. Qed.
+
+End Tactics.
+
 End ModelLogic.
+
+  Ltac cwp_bind_core K :=
+    lazymatch eval hnf in K with
+    | [] => idtac
+    | _ => eapply (tac_cwp_bind K); [simpl; reflexivity|reduction.pm_prettify]
+    end.
+
+  Tactic Notation "cwp_bind" open_constr(efoc) :=
+    iStartProof;
+    lazymatch goal with
+    | |- envs_entails _
+          (* (wp ?s ?E ?locale ?e ?Q) *)
+          (cwp ?e ?Φ ?s ?ε__wp ?ε__lift ?τ ?ρ)
+         =>
+        first [ reshape_expr e ltac:(fun K e' => unify e' efoc; cwp_bind_core K)
+              | fail 1 "cwp_bind: cannot find" efoc "in" e ]
+    | _ => fail "cwp_bind: not a 'wp'"
+  end.
+
+  
 
 
 Section Test.
@@ -187,6 +230,17 @@ Section Test.
   Notation "tid ↦M R" := (partial_mapping_is {[ tid := R ]}) (at level 33).
   Notation "tid ↦m ρ" := (partial_mapping_is {[ tid := {[ ρ ]} ]}) (at level 33).
   Notation "ρ ↦F f" := (partial_fuel_is {[ ρ := f ]}) (at level 33).
+
+  Definition prog: expr heap_lang :=
+    let: "x" := ref #2 in
+    "x" <- #1. 
+
+  Lemma bind_test s E ε__lift tid g: ⊢ CWP prog (fun _ => ⌜ False ⌝) s E ε__lift tid g.
+  Proof. 
+    iStartProof. rewrite /prog.
+    rewrite /CWP.
+    cwp_bind (ref #2)%E.
+  Abort. 
 
 Lemma wp_step_model s tid ρ (f1 : nat) fs fr s1 s2 E ε__lift e Φ (g: G):
   TCEq (to_val e) None →
