fairness/examples/comp/lib_interface.v
@@ -1,0 +1,36 @@
+From iris.bi Require Import bi.
+From trillium.fairness.heap_lang Require Import lang.
+From trillium.fairness Require Import fairness.
+From trillium.fairness.ext_models Require Import ext_models.
+
+Section LibInterface.
+
+  Definition in_dom_rel {A: Type} (R: relation A) :=
+    fun x => exists y, R x y. 
+
+  Definition in_cod_rel {A: Type} (R: relation A) :=
+    fun y => exists x, R x y. 
+
+  Class LibInterface := {
+      libM: FairModel;
+      libEM: ExtModel libM (fmrole libM);
+      lib_step_ex_dec :> forall st ρ, Decision (exists st', fmtrans libM st (Some ρ) st');
+      reset_lib := @ETs _ _ libEM;
+      lib_reset_dom: forall ρ st, in_dom_rel (reset_lib ρ) st <-> ¬ role_enabled_model ρ st;
+      lib_strong_lr: FM_strong_lr libM;
+
+      libGSPre: gFunctors -> Set;
+      libGS: gFunctors -> Set;
+      lib_msi `{libGS Σ}: fmstate libM -> iProp Σ;
+      lib_fun: val heap_lang;
+      lib_pre `{libGS Σ}: fmrole libM -> iProp Σ;
+      lib_post `{libGS Σ}: fmrole libM -> iProp Σ;
+      lib_st0: fmstate libM;
+      lib_init `{l0: libGSPre Σ}: ⊢ ∀ ρ, |==> ∃ (l: libGS Σ), lib_msi lib_st0 (libGS0 := l) ∗ lib_post ρ (libGS0 := l);
+      lib_post_dis `{l: libGS Σ}: ⊢ ∀ ρ st, lib_msi st (libGS0 := l) ∗ lib_post ρ (libGS0 := l) → ⌜ ¬ role_enabled_model ρ st ⌝;
+      lib_reset `{l: libGS Σ}:
+        ⊢ ∀ st ρ, lib_msi st (libGS0 := l) ∗ lib_post ρ (libGS0 := l) ==∗
+                   ∃ st', lib_msi st' (libGS0 := l) ∗ lib_pre ρ (libGS0 := l);
+  }.
+
+End LibInterface.
